progress on kyberslash proof

bedrock2/src/bedrock2Examples/kyberslash.v
@@ -26,28 +26,34 @@ void poly_tomsg(uint8_t msg[KYBER_INDCPA_MSGBYTES], const poly *a)
 }
  *)
 
-Require Import BinIntDef coqutil.Word.Interface coqutil.Word.Bitwidth.
-Require Import Coq.ZArith.BinInt Coq.Strings.String Coq.Lists.List. Import ListNotations.
-Require Import coqutil.Macros.subst coqutil.Macros.unique bedrock2.Syntax.
-Require Import bedrock2.NotationsCustomEntry.
-Require Import coqutil.sanity.
+Require Import Coq.Strings.String Coq.ZArith.ZArith.
+Require Import coqutil.Z.Lia.
+From bedrock2 Require Import NotationsCustomEntry ProgramLogic Map.Separation Map.SeparationLogic Array Scalars Loops.
 
-Local Open Scope Z_scope. Local Open Scope string_scope. Local Open Scope list_scope.
-Require Import bedrock2.Syntax.
-Import Syntax.bopname. Print expr.expr. Print mul.
 
-Infix "/" := (expr.op divu) (in custom bedrock_expr at level 5, left associativity).
+From coqutil Require Import Datatypes.List Word.Bitwidth Word.Interface Map.Interface. (* coercions word and rep *)
+From bedrock2 Require Import Semantics Syntax.
+Import coqutil.Word.Properties coqutil.Map.Properties.
+
+Require Import bedrock2.AbsintWordToZ.
+
+Infix "/" := (expr.op bopname.divu) (in custom bedrock_expr at level 5, left associativity).
 
 Section WithWord.
-  (*Context {width: Z}{BW: Bitwidth width}{word: word.word width}.*)
-  Context {word: word.word 32}.
-  Context (KYBER_N KYBER_Q : word).
-  (* ^is this how to do global constants in bedrock2? *)
+  Context {width: Z} {BW: Bitwidth width}. (*{word: word.word w*)
+  Context {word: word.word width}.
+  Context {mem: map.map word Byte.byte}.
+  Context {locals: map.map string word}.
+  Context {env : map.map string (list string * list string * cmd)}.
+  Context {word_ok: word.ok word} {mem_ok: map.ok mem} {locals_ok: map.ok locals} {env_ok : map.ok env}.
+  Context {ext_spec: ExtSpec} {ext_spec_ok : ext_spec.ok ext_spec}.
+  Context (KYBER_N KYBER_Q KYBER_INDCPA_MSGBYTES : Z).
+  (* ^is this how to do global constants in bedrock2? *) Print expr.expr.
   
   Definition poly_tomsg :=
     func! (msg, a_coeffs) {
         i = $0;
-        while (i < KYBER_N / $8) {
+        while (i < coq:(expr.literal KYBER_N) / $8) {
             store1(msg + i, $0);
             j = $0;
             while (j < $8) {
@@ -64,7 +70,7 @@ Section WithWord.
           }
       }.
   
-  Definition bad_poly_tomsg :=
+  (*Definition bad_poly_tomsg :=
     func! (msg, a_coeffs) {
         i = $0;
         while (i < KYBER_N / $8) {
@@ -87,44 +93,155 @@ Section WithWord.
               };
             i = i + $1
           }
-      }.
+      }.*)
 
-  Require Import bedrock2.NotationsCustomEntry coqutil.Macros.WithBaseName.
-
-  Import Syntax BinInt String List.ListNotations.
-  Local Open Scope string_scope. Local Open Scope Z_scope. Local Open Scope list_scope.
-  
-
-  Require Import bedrock2.WeakestPrecondition.
-  Require Import bedrock2.Semantics bedrock2.FE310CSemantics.
-  Require Import coqutil.Map.Interface bedrock2.Map.Separation bedrock2.Map.SeparationLogic.
-  From bedrock2 Require Import NotationsCustomEntry ProgramLogic Map.Separation Array Scalars Loops.
-
-  
-  Require Import bedrock2.WeakestPreconditionProperties.
-  From coqutil.Tactics Require Import Tactics letexists eabstract.
-  Require Import bedrock2.ProgramLogic bedrock2.Scalars.
-  Require Import coqutil.Word.Interface.
-  
-  Section WithParameters.
-    Context {mem: map.map word Byte.byte}.
-    Context {word_ok: word.ok word} {mem_ok: map.ok mem}. Print array. Print ptsto. Print scalar16. Print ptsto.
-  
-    Definition poly_tomsg_ct : spec_of "poly_tomsg" :=
+    Instance poly_tomsg_ct : spec_of "poly_tomsg" :=
       fun functions =>
-        exists f : word -> word -> trace,
+        exists f : word -> word -> Z -> trace,
         forall (k : trace) (t : io_trace) (m : mem) (msg a_coeffs : word) (msg_vals : list Byte.byte) (a_coeffs_vals : list word) (R : mem -> Prop),
           ((array scalar8 (word.of_Z 1) msg msg_vals) ⋆ (array scalar16 (word.of_Z 2) a_coeffs a_coeffs_vals) ⋆ R)%sep m ->
-          True.
-    (*(scalar a_addr a ⋆ scalar b_addr b ⋆ R)%sep m ->
-          call functions "swap" k t m [a_addr; b_addr]
+          List.length a_coeffs_vals = Z.to_nat KYBER_N ->
+          List.length msg_vals = Z.to_nat KYBER_INDCPA_MSGBYTES ->
+          @word.unsigned _ word (word.divu (word.of_Z KYBER_N) (word.of_Z 8)) <= KYBER_INDCPA_MSGBYTES ->
+          WeakestPrecondition.call functions "poly_tomsg" k t m (msg :: a_coeffs :: nil)
             (fun (k' : trace) (T : io_trace) (M : mem) (rets : list word) =>
-               M =* scalar a_addr b * scalar b_addr a * R /\ T = t /\ rets = [] /\
+               T = t /\ rets = nil /\
                  exists k'',
-                   k' = k'' ++ k /\ k'' = f a_addr b_addr
-            ).*)
+                   k' = app k'' k /\ k'' = f msg a_coeffs KYBER_N).
 
+    Require Import bedrock2.ZnWords.
 
+    
+    Lemma poly_tomsg_ok : program_logic_goal_for_function! poly_tomsg.
+    Proof.
+      repeat straightline. Check @Loops.tailrec.
+      refine ((Loops.tailrec
+                 (* types of ghost variables*) (let c := HList.polymorphic_list.cons in c _ (c _ HList.polymorphic_list.nil))
+                 (* program variables *) ("i" :: "a_coeffs" :: "msg" :: nil))%string
+                (fun vi msg_vals a_coeffs_vals k t m i a_coeffs msg =>
+                   PrimitivePair.pair.mk
+                     (List.length a_coeffs_vals = Z.to_nat KYBER_N /\
+                      List.length msg_vals = Z.to_nat KYBER_INDCPA_MSGBYTES /\
+                        ((array scalar8 (word.of_Z 1) msg msg_vals) * (array scalar16 (word.of_Z 2) a_coeffs a_coeffs_vals) * R)%sep m 
+                       /\ vi = @word.unsigned _ word (word.divu (word.of_Z KYBER_N) (word.of_Z 8)) - word.unsigned i) (* precondition *)
+                     (fun K T M I A_COEFFS MSG => (*postcondition*) 
+                        T = t /\ A_COEFFS = a_coeffs /\ MSG = msg)) 
+                (fun n m => 0 <= n < m) (* well_founded relation *)
+                _ _ _ _ _ _ _);
+        cbn [HList.hlist.foralls HList.tuple.foralls
+               HList.hlist.existss HList.tuple.existss
+               HList.hlist.apply  HList.tuple.apply
+               HList.hlist
+               List.repeat Datatypes.length
+               HList.polymorphic_list.repeat HList.polymorphic_list.length
+               PrimitivePair.pair._1 PrimitivePair.pair._2] in *.
+      { cbv [Loops.enforce]; cbn.
+          subst l l0.
+          repeat (rewrite ?map.get_put_dec, ?map.get_remove_dec; cbn). split.
+          { exact eq_refl. }
+          { eapply map.map_ext; intros k0.
+            repeat (rewrite ?map.get_put_dec, ?map.get_remove_dec, ?map.get_empty; cbn -[String.eqb]).
+            repeat (destruct String.eqb; trivial). } }
+      { exact (Z.lt_wf _). }
+      { repeat (straightline || intuition eauto). }
+      { repeat straightline.
+        eexists. eexists. split.
+        { repeat straightline. eexists. split.
+          { repeat straightline. subst localsmap. cbv [reconstruct].
+            cbn [HList.tuple.of_list]. cbv [map.putmany_of_tuple]. simpl.
+            Search (map.get (map.put _)). Search map.get. rewrite map.get_put_same.
+            reflexivity. (* why will straightline not do that for me??
+                            it would earlier, but then I changed some context variables. *) }
+          repeat straightline. }
+        repeat straightline.
+        split. 2: auto.
+        repeat straightline.
+        eexists. eexists. split.
+        { repeat straightline. eexists. split.
+          { repeat straightline. subst localsmap. cbv [reconstruct].
+            cbn [HList.tuple.of_list]. cbv [map.putmany_of_tuple]. simpl.
+            rewrite map.get_put_diff by congruence. rewrite map.get_put_diff by congruence.
+            rewrite map.get_put_same.
+            reflexivity. }
+          repeat straightline. eexists. split.
+          { subst localsmap. cbv [reconstruct].
+            cbn [HList.tuple.of_list]. cbv [map.putmany_of_tuple]. simpl.
+            rewrite map.get_put_same. reflexivity. }
+          eauto. }
+        repeat straightline.
+        (*finally we do something interesting*)
+        eapply Scalars.store_one_of_sep.
+        { Check (array_address_inbounds ptsto (word.of_Z 1) x x3 (word.add x3 x1)). Search Init.Byte.byte.
+          destruct (word.ltu x1 _) eqn:E.
+          2: { rewrite word.unsigned_of_Z_0 in H6. exfalso. auto. }
+          rewrite word.unsigned_ltu in E. apply Z.ltb_lt in E.
+          Check @array_index_nat_inbounds.
+           seprewrite_in (@array_index_nat_inbounds _ _ _ _ _ _ _ ptsto (word.of_Z 1) Byte.x00 x x3 (Z.to_nat (word.unsigned x1))) H5. Search x.
+          { ZnWords. }
+          replace (@word.of_Z _ word (@word.unsigned _ word (word.of_Z 1) * Z.of_nat (Z.to_nat (word.unsigned x1)))) with x1 in *.
+          2: { Search (Z.of_nat (Z.to_nat _)). rewrite Z2Nat.id.
+               2: { assert (Hnonneg := word.unsigned_range x1 ). blia. }
+               Search (word.unsigned _ * word.unsigned _). Search word.unsigned.
+               apply word.unsigned_inj. Search (word.unsigned (word.of_Z _)).
+               repeat rewrite word.unsigned_of_Z. cbv [word.wrap].
+               Search ((_ mod _ * _) mod _).
+               rewrite Z.mul_mod_idemp_l.
+               2: { Search (_ ^ _ <> 0). apply word.modulus_nonzero. }
+               assert (Hx1 := word.unsigned_range x1).
+               Search (?a mod ?b = ?a). rewrite Z.mod_small; blia. }
+          ecancel_assumption. }
+        repeat straightline. (* neat, why did that work now? *)
+        
+          
+          
+               { blia. }
+               { blia.
+                 { 
+               Search ord.unsigned.
+               ZnWords.
+               cbv [word.of_Z]. rewrite <- word.unsigned_mul.
+
+               rewrite Z2Nat.inj_le. rite Z.of_nat_inj. ZnWords.
+            2: { Search (Z.to_nat _ <= Z.to_nat _)%nat. apply Z2Nat.inj_le.
+                 3: { 
+            { eassumption.
+            rewrite word.word_sub_add_l_same_l. ZnWords. }
+          { rewrite word.word_sub_add_l_same_l. Search (_ mod 1). rewrite word.unsigned_of_Z.
+            cbv [word.wrap]. Search array. Search (_ mod (_ mod _)). apply Z.mod_1_r. ZnWords.
+          
+            rewrite H4. clear H4. ZnWords. rewrite Z2Nat.id. ZnWords.
+            2: { Search word.unsigned.
+                 assert (Hnonneg := word.unsigned_range (word.divu (word.of_Z KYBER_N) (word.of_Z 8)) ).
+                 blia. }
+            Search word.unsigned. ZnWords.
+            remember (word.divu _ _) as z eqn:Heqz.
+            rewrite word.unsigned_of_Z in *. cbv [word.wrap] in *. Search (1 mod _).
+            ZnWords. }
+            clear Heqz. Search word.wrap. Print word.wrap. Check array_address_inbounds.
+            (*this is not nice. maybe try writing tailrec as in memequal, where we ignore the part of *)
+             blia.
+            Search word.divu. blia. 
+            simpl in E. rewrite word.of_Z_unsigned in E. slia.
+            discriminate H4. destruct H4. congruence.
+            Search (word.unsigned (word.of_Z _)).
+            blia.
+          4: {
+        fold (@word.unsigned _ word).
+        econstructor. split.
+        { Check Scalars.store_one_of_sep.
+        straightline. eexists. eexists. split.
+        { repeat straightline.
+      refine (
+          tailrec (HList.polymorphic_list.cons _ (HList.polymorphic_list.cons _ HList.polymorphic_list.nil)) ("left"::"right"::"target"::nil)%list%string
+            (fun l xs R k t m left right target =>
+               PrimitivePair.pair.mk
+                 (sep (array scalar (word.of_Z 8) left xs) R m /\
+                    \_ (right ^- left) = 8*Z.of_nat (Datatypes.length xs) /\
+                    List.length xs = l)
+                 (fun        K T M LEFT RIGHT TARGET => T = t /\ sep (array scalar (word.of_Z 8) left xs) R M))
+            lt _ _ _ _ _ _ _)
+               
+Print bsearch.
 
 (*Instance spec_of_bsearch : spec_of "bsearch"%string := fun functions =>
   forall left right target xs R k t m,
